twilight for get_eq proof

verif/trie/functional/cursored_kv.v
@@ -1,6 +1,7 @@
 (** * cursored_kv.v: Interface and Specification for general KV Store with ordered keys and cursors*)
 Require Import Coq.Structures.OrderedTypeEx.
 Require Import Coq.Structures.OrderedType.
+Require Import Coq.FSets.FMapInterface.
 Require Import VST.floyd.proofauto.
 Require Import DB.common.
 Require Import DB.functional.kv.
@@ -8,24 +9,29 @@ Require Import DB.functional.kv.
 (* This file is mainly based on Brian's paper and his BTreesModule.v, with some improvement and generalization *)
 (* Also, this file takes the FMap Module as reference for interface *)
 Module Type ABSTRACT_TABLE (KeyType: UsualOrderedType).
-
   Definition key := KeyType.t.
   Hint Transparent key.
   Parameter table: Type -> Type.
   Parameter cursor: Type -> Type.
+  Parameter allocator: Type.
 
   Section Types.
     Context {elt: Type}.
-    Parameter empty: table elt.
+    (* Predicate rather than variable because of possible addresses in the data type *)
+    Parameter empty: allocator -> table elt * allocator.
 
     (* Functions *)
+    (* Sematics: cursor should point to a place where to the left, all keys are less than the key,
+     * to the right, all keys are no less than the key *)
+    (* Therefore [make_cursor] should always return one, but not always the expected one *)
     Parameter make_cursor: key -> table elt -> cursor elt.
-    (* no more get_table, cause they are separated defs now *)
+    (* By [get] functions, we always access the first key to the right *)
+    Parameter get: cursor elt -> table elt -> option (key * elt).
     Parameter get_key: cursor elt -> table elt -> option key.
-    Parameter get: cursor elt -> table elt -> option elt.
+    Parameter get_value: cursor elt -> table elt -> option elt.
     (* we do expect that the cursor is moved when insertion is performed,
      * but where it is afterwards remains to be discussed *)
-    Parameter put: cursor elt -> elt -> table elt -> cursor elt * table elt.
+    Parameter put: key -> elt -> cursor elt -> table elt * allocator -> cursor elt * (table elt * allocator).
     Parameter next_cursor: cursor elt -> table elt -> cursor elt.
     Parameter prev_cursor: cursor elt -> table elt -> cursor elt.
     Parameter first_cursor: table elt -> cursor elt.
@@ -34,75 +40,86 @@ Module Type ABSTRACT_TABLE (KeyType: UsualOrderedType).
     (* TODO: do we need a [move_cursor]?
      * From the client's view, it does not matter whether it is [make] or [move], but it might increase
      * difficulty in proof *)
-    Parameter move_cursor: key -> cursor elt -> table elt -> cursor elt.
+    (* Parameter move_cursor: key -> cursor elt -> table elt -> cursor elt. *)
 
-
-    (* Correctness Relations *)
-    (* originally [abs_rel], meaning that the table and the cursor are binded together (might need better name) *)
+    (* Relations between keys, cursors and tables *)
+    (* [abs_rel] means that the table and the cursor are binded together (might need better name) *)
     (* In implementation, it's translated to correct cursor with get tree from cursor works *)
-    Parameter bind_rel: cursor elt -> table elt -> Prop.
-    (* Do we need this? This just sounds like [bind_rel c t /\ get_key c t = Some k] *)
+    Parameter abs_rel: cursor elt -> table elt -> Prop.
+    (* Do we need this? This just sounds like [abs_rel c t /\ get_key c t = Some k] *)
+    (* Not true, in btree, the cursor created with non-existing keys will not return the key with [get_key],
+     * but rather, a bunch of keys can still be associated with the cursor *)
     Parameter key_rel: key -> cursor elt -> table elt -> Prop.
-    (* DO we need this again? What about [bind_rel c1 t /\ bind_rel c2 t /\ get_key c1 t = get_key c2 t] *)
+    (* DO we need this again? What about [abs_rel c1 t /\ abs_rel c2 t /\ get_key c1 t = get_key c2 t] *)
     Parameter eq_cursor : cursor elt -> cursor elt -> table elt -> Prop.
+    (* Definition eq_cursor (c1 c2: cursor elt) (t: table elt) := *)
+    (*   abs_rel c1 t /\ abs_rel c2 t /\ get_key c1 t = get_key c2 t. *)
     (* What do we need to ensure about the previous two definition? Should they be transitive? *)
-    (* This might make sense since *)
     Parameter cursor_correct: cursor elt -> Prop.
     Parameter table_correct: table elt -> Prop.
 
     Section Specs.
       Variable t: table elt.
-      Variable c c1 c2 c3: cursor elt.
+      Variable c c1 c2 c3: cursor elt. 
       Variable k k1 k2 k3: key.
       Variable e e1 e2: elt.
-      Hypothesis Htable_correct: table_correct t.
+      Variable a: allocator.
+
+      Axiom abs_correct: abs_rel c t -> (cursor_correct c <-> table_correct t).
+
       (* table-cursor relations *)
       (* We need to make sure that the cursor and the table are actually working with each other *)
-      Axiom make_cusor_binded: bind_rel (make_cursor k t) t.
-      Axiom put_bind:
-        let (new_cursor, new_table) := put c e t in
-        bind_rel new_cursor new_table.
+      (* This is actually implied by [make_cursor_key] *)
+      (* Axiom make_cusor_abs: abs_rel (make_cursor k t) t. *)
+      (* Do we need this? *)
+      (* Axiom put_abs: *)
+      (*   let (new_cursor, new_table) := put c e t in *)
+      (*   abs_rel new_cursor new_table. *)
       (* TODO: What about at the end of range? *)
-      Axiom next_cursor_bind: bind_rel c t -> bind_rel (next_cursor c t) t.
-      Axiom prev_cursor_bind: bind_rel c t -> bind_rel (prev_cursor c t) t.
-      Axiom first_cursor_bind: bind_rel (first_cursor t) t.
-      Axiom last_cursor_bind: bind_rel (last_cursor t) t.
-      Axiom move_cursor_bind: bind_rel c t -> bind_rel (move_cursor k c t) t.
-
-      (* TODO: is this proper? *)
-      Axiom key_bind: key_rel k c t -> bind_rel c t.
+      Axiom next_cursor_abs: abs_rel c t -> abs_rel (next_cursor c t) t.
+      Axiom prev_cursor_abs: abs_rel c t -> abs_rel (prev_cursor c t) t.
+      Axiom first_cursor_abs: table_correct t -> abs_rel (first_cursor t) t.
+      Axiom last_cursor_abs: table_correct t -> abs_rel (last_cursor t) t.
+      (* Axiom move_cursor_abs: abs_rel c t -> abs_rel (move_cursor k c t) t. *)
 
       (* permute of get and insert operations *)
-      (* Assume [key_rel] does entail [bind_rel] *)
+      (* Assume [key_rel] does entail [abs_rel] *)
       Axiom get_put_same:
-        key_rel k c1 (snd (put c2 e t)) ->
-        key_rel k c2 t ->
-        get c1 (snd (put c2 e t)) = Some e.
+        abs_rel c1 t ->
+        abs_rel c2 t -> (* doubtful *)
+        key_rel k c1 (fst (snd (put k e c2 (t, a)))) ->
+        get c1 (fst (snd (put k e c2 (t, a)))) = Some (k, e).
       Axiom get_put_diff:
         k1 <> k2 ->
-        key_rel k1 c1 (snd (put c2 e t)) ->
-        key_rel k2 c2 t ->
+        table_correct t ->
+        cursor_correct c2 ->
+        key_rel k1 c1 (fst (snd (put k2 e c2 (t, a)))) ->
         key_rel k1 c3 t ->
-        get c1 (snd (put c2 e t)) = get c3 t.
+        get c1 (fst (snd (put k2 e c2 (t, a)))) = get c3 t.
 
       (* get in specific conditions *)
       Axiom get_last:
         get (last_cursor t) t = None.
-      Axiom get_empty:
-        get c empty = None.
+      Axiom get_empty: 
+        abs_rel c (fst (empty a)) -> get c (fst (empty a)) = None.
 
-      (* Cursor creation and keys *)
+      (* Cursor and keys *)
+
+      Axiom key_rel_eq_cursor:
+        key_rel k c1 t ->
+        key_rel k c2 t ->
+        abs_rel c1 t ->
+        abs_rel c2 t ->
+        eq_cursor c1 c2 t.
 
       Axiom make_cursor_key:
         key_rel k (make_cursor k t) t.
-      Axiom move_cursor_key:
-        key_rel k (move_cursor k c t) t.
-
+      
       (* cursor movement with respect to the order of key *)
       Axiom next_prev:
-        bind_rel c t -> ~ eq_cursor c (last_cursor t) t -> eq_cursor c (prev_cursor (next_cursor c t) t) t.
+        abs_rel c t -> ~ eq_cursor c (last_cursor t) t -> eq_cursor c (prev_cursor (next_cursor c t) t) t.
       Axiom prev_next:
-        bind_rel c t -> ~ eq_cursor c (first_cursor t) t -> eq_cursor c (next_cursor (prev_cursor c t) t) t.
+        abs_rel c t -> ~ eq_cursor c (first_cursor t) t -> eq_cursor c (next_cursor (prev_cursor c t) t) t.
       Axiom next_order:
         ~ eq_cursor c (last_cursor t) t -> key_rel k1 c t -> key_rel k2 (next_cursor c t) t -> KeyType.lt k1 k2.
       Axiom prev_order:
@@ -120,6 +137,1072 @@ Module Type ABSTRACT_TABLE (KeyType: UsualOrderedType).
   End Types.
 End ABSTRACT_TABLE.
 
+Module AbstractTableFacts (KeyType: UsualOrderedType) (AbstractTable: ABSTRACT_TABLE KeyType).
+  Import AbstractTable.
+
+  Section Implication.
+    Context {elt: Type}.
+    Variable t: table elt.
+    Variable c c1 c2 c3: cursor elt.
+    Variable k k1 k2 k3: key.
+    Variable e e1 e2: elt.
+
+    (* Lemma key_abs: *)
+    (*   key_rel k c t -> abs_rel c t. *)
+    (* Proof. *)
+    (*   intros. *)
+    (*   destruct H. *)
+    (*   assumption. *)
+    (* Qed. *)
+
+    (* Lemma eq_cursor_refl: *)
+    (*   abs_rel c t -> eq_cursor c c t. *)
+    (* Proof. *)
+    (*   unfold eq_cursor. *)
+    (*   split3; auto. *)
+    (* Qed. *)
+  End Implication.
+End AbstractTableFacts.
+
+Module SortedListTable (KeyType: UsualOrderedType) <: ABSTRACT_TABLE KeyType.
+  Definition key := KeyType.t.
+  Definition table (elt: Type) := list (key * elt).
+  Definition cursor (elt: Type) := Z.
+  Definition allocator := unit.
+
+  Module KeyFacts := OrderedTypeFacts KeyType.
+
+  Import ListNotations.
+  Section Types.
+    Context {elt: Type}.
+    (* Predicate rather than variable because of possible addresses in the data type *)
+    Definition empty (tt: allocator): table elt * allocator :=
+      ([], tt).
+
+    Fixpoint make_cursor (k: key) (t: table elt): cursor elt :=
+      match t with
+      | [] => 0
+      | (k', _) :: t' =>
+        if KeyFacts.lt_dec k' k then
+          1 + make_cursor k t'
+        else
+          0
+      end.
+
+    Instance option_key_inh: Inhabitant (option key) := None.
+    Instance option_elt_inh: Inhabitant (option elt) := None.
+    Instance option_binding_inh: Inhabitant (option (key * elt)) := None.
+
+    Definition get (c: cursor elt) (t: table elt): option (key * elt) :=
+      Znth c (map Some t).
+
+    Definition get_key (c: cursor elt) (t: table elt): option key :=
+      match get c t with
+      | Some (k, _) => Some k
+      | None => None
+      end.
+
+    Definition get_value (c: cursor elt) (t: table elt): option elt :=
+      match get c t with
+      | Some (_, v) => Some v
+      | None => None
+      end.
+
+    Fixpoint put_aux (k: key) (v: elt) (t: table elt) :=
+      match t with
+      | (k', v') :: l' =>
+        if KeyFacts.lt_dec k k' then
+          (k, v) :: (k', v') :: l'
+        else
+          if KeyFacts.eq_dec k k' then
+            (k, v) :: l'
+          else
+            (k', v') :: (put_aux k v l')
+      | nil => (k, v) :: nil
+      end.
+
+    Definition put (k: key) (v: elt) (c: cursor elt) (table_with_allocator: table elt * allocator) :=
+      let (t, a) := table_with_allocator in
+      (c, (put_aux k v t, tt)).
+
+    Definition next_cursor (c: cursor elt) (t: table elt) :=
+      if Z_lt_dec c (Zlength t) then c + 1 else c.
+    Definition prev_cursor (c: cursor elt) (t: table elt) :=
+      if Z_gt_dec c 0 then c - 1 else c.
+    Definition first_cursor (t: table elt) := 0.
+    Definition last_cursor (t: table elt) := Zlength t.
+    
+    Definition key_rel (k: key) (c: cursor elt) (t: table elt) := forall c',
+      (0 <= c' < c -> exists k', get_key c' t = Some k' /\ KeyFacts.TO.lt k' k) /\
+      (c <= c' < Zlength t -> exists k', get_key c' t = Some k' /\ ~ KeyFacts.TO.lt k' k).
+
+    Definition eq_cursor (c1 c2: cursor elt) (t: table elt) := c1 = c2.
+    Definition cursor_correct (c: cursor elt) := True.
+    Definition table_correct (t: table elt) := Sorted KeyType.lt (map fst t).
+    Definition abs_rel (c: cursor elt) (t: table elt) := table_correct t /\ 0 <= c <= Zlength t.
+
+    Section Specs.
+      Theorem abs_correct: forall c t,
+        abs_rel c t -> cursor_correct c /\ table_correct t.
+      Proof. firstorder. Qed.
+
+      Theorem next_cursor_abs: forall c t,
+          abs_rel c t -> abs_rel (next_cursor c t) t.
+      Proof.
+        (* This does not necessarily make sense at the end *)
+        unfold abs_rel; unfold next_cursor; intros ? ? [].
+        split; auto.
+        split.
+        - if_tac; omega.
+        - if_tac.
+          + omega.
+          + omega.
+      Qed.
+
+      Theorem prev_cursor_abs: forall c t,
+          abs_rel c t -> abs_rel (prev_cursor c t) t.
+      Proof.
+        (* This does not necessarily make sense at the end *)
+        unfold abs_rel; unfold prev_cursor; intros ? ? [].
+        split; auto.
+        split.
+        - if_tac; omega.
+        - if_tac.
+          + omega.
+          + omega.
+      Qed.
+
+      Theorem first_cursor_abs: forall t,
+          table_correct t -> abs_rel (first_cursor t) t.
+      Proof.
+        unfold abs_rel; unfold first_cursor; intros.
+        split;
+          [ auto | list_solve ].
+      Qed.
+        
+      Theorem last_cursor_abs: forall t,
+          table_correct t -> abs_rel (last_cursor t) t.
+      Proof.
+        unfold abs_rel; unfold last_cursor; intros.
+        split;
+          [ auto | list_solve ].
+      Qed.
+      
+      Theorem get_last: forall t,
+          get (last_cursor t) t = None.
+      Proof.
+        unfold get, last_cursor; intros.
+        rewrite Znth_overflow.
+        - reflexivity.
+        - rewrite Zlength_map.
+          rep_omega.
+      Qed.
+
+      Lemma table_correct_strong: forall t,
+          table_correct t <-> StronglySorted KeyType.lt (map fst t).
+      Proof.
+        split; intros.
+        - apply Sorted_StronglySorted;
+            [ unfold Relations_1.Transitive; apply KeyType.lt_trans | auto ].
+        - apply StronglySorted_Sorted.
+          assumption.
+      Qed.
+
+      Lemma get_inrange: forall c t,
+          abs_rel c t -> ~ eq_cursor (last_cursor t) c t -> exists kv, get c t = Some kv.
+      Proof.
+        unfold abs_rel, eq_cursor, last_cursor, get; intros.
+        assert (0 <= c < Zlength t) by (change (cursor elt) with Z in *; list_solve).
+        pose proof (Znth_In c (map Some t) ltac:(rewrite Zlength_map; list_solve)).
+        destruct (Znth c (map Some t)) eqn:Heqn.
+        + exists p.
+          reflexivity.
+        + clear H H0 H1 Heqn.
+          exfalso.
+          induction t.
+          * inversion H2.
+          * inversion H2; congruence.
+      Qed.
+
+      Lemma get_ge: forall k1 k2 c t,
+        abs_rel c t -> key_rel k1 c t -> get_key c t = Some k2 -> ~ KeyFacts.TO.lt k2 k1.
+      Proof.
+        unfold abs_rel, key_rel, get_key; intros.
+        specialize (H0 c) as [_ ?].
+        destruct (eq_dec c (last_cursor t)).
+        + subst.
+          rewrite get_last in H1.
+          congruence.
+        + unfold last_cursor in n.
+          specialize (H0 ltac:(change (cursor elt) with Z in *; omega)) as [k2' []].
+          rewrite H1 in H0.
+          inversion H0.
+          assumption.
+      Qed.
+
+      Theorem key_rel_eq_cursor: forall k c1 c2 t,
+        key_rel k c1 t -> key_rel k c2 t ->
+        abs_rel c1 t -> abs_rel c2 t ->
+        eq_cursor c1 c2 t.
+      Proof.
+        unfold key_rel; unfold abs_rel; unfold eq_cursor.
+        intros.
+        destruct (eq_dec c1 c2); [ assumption | ].
+        assert (c1 < c2 \/ c1 > c2) by (change (cursor elt) with Z in *; omega); clear n; destruct H3.
+        - specialize (H0 c1) as [? _].
+          specialize (H0 ltac:(omega)) as [k0 []].
+          pose proof (get_ge k k0 c1 t H1 H H0).
+          KeyFacts.order.
+        - specialize (H c2) as [? _].
+          specialize (H ltac:(omega)) as [k0 []].
+          pose proof (get_ge k k0 c2 t H2 H0 H).
+          KeyFacts.order.
+      Qed.
+
+      Lemma make_cursor_inrange: forall k t,
+          0 <= make_cursor k t <= Zlength t.
+      Proof.
+        intros; unfold make_cursor.
+        induction t as [ | [] ?]; intros.
+        - rewrite Zlength_nil; omega.
+        - if_tac.
+          + rewrite Zlength_cons.
+            omega.
+          + list_solve.
+      Qed.
+
+      Lemma make_cursor_continuous: forall k t k' v',
+          make_cursor k t <= make_cursor k (t ++ [(k', v')]) <= make_cursor k t + 1.
+      Proof.
+        induction t as [ | [] ?]; intros; simpl.
+        - if_tac; omega.
+        - specialize (IHt k' v').
+          if_tac; omega.
+      Qed.
+
+      Theorem make_cursor_abs: forall k t,
+          table_correct t -> abs_rel (make_cursor k t) t.
+      Proof.
+        induction t as [ | [] ?]; intros; simpl.
+        - split; auto.
+          rewrite Zlength_nil; omega.
+        - split; auto.
+          pose proof (make_cursor_inrange k t).
+          if_tac.
+          + rewrite Zlength_cons.
+            omega.
+          + rewrite Zlength_cons.
+            omega.
+      Qed.
+
+      Theorem make_cursor_key: forall k t,
+          table_correct t -> key_rel k (make_cursor k t) t.
+      Proof.
+        unfold key_rel, make_cursor, get_key, get.
+        (* intros k t. *)
+        (* generalize dependent k. *)
+        (* pattern t. *)
+        induction t as [ | [] ?]; intros.
+        - split; intros.
+          + omega.
+          + rewrite Zlength_nil in H0; omega.
+        - split; intros; fold make_cursor in *.
+          + if_tac in H0.
+            * inv H.
+              specialize (IHt ltac:(auto) (c' - 1)) as [? _].
+              destruct (eq_dec c' 0).
+              -- subst.
+                 simpl.
+                 exists k0.
+                 auto.
+              -- specialize (H ltac:(omega)) as [k' []].
+                 simpl.
+                 rewrite Znth_pos_cons by omega.
+                 exists k'.
+                 rewrite H.
+                 auto.
+            * omega.
+          + if_tac in H0.
+            * inv H.
+              specialize (IHt ltac:(auto) (c' - 1)) as [_ ?].
+              rewrite Zlength_cons in H0.
+              specialize (H ltac:(omega)) as [k' []].
+              exists k'.
+              simpl.
+              pose proof (make_cursor_inrange k t).
+              rewrite Znth_pos_cons by omega.
+              rewrite H.
+              auto.
+            * destruct (Znth c' (map Some ((k0, e) :: t))) eqn:Heqn.
+              -- destruct p.
+                 exists k1.
+                 split; auto.
+                 apply table_correct_strong in H.
+                 inv H.
+                 destruct (eq_dec c' 0).
+                 ++ subst.
+                    simpl in Heqn.
+                    rewrite Znth_0_cons in Heqn.
+                    inv Heqn.
+                    KeyFacts.order.
+                 ++ rewrite Forall_forall in H5.
+                    simpl in Heqn.
+                    rewrite Znth_pos_cons in Heqn by omega.
+                    rewrite Zlength_cons in H0.
+                    pose proof (Znth_In (c' - 1) (map Some t) ltac:(list_solve)).
+                    assert (In k1 (map fst t)). {
+                      rewrite Heqn in H.
+                      clear -H.
+                      induction t.
+                      - simpl in H.
+                        auto.
+                      - inv H.
+                        + inv H0.
+                          simpl.
+                          auto.
+                        + simpl.
+                          right.
+                          auto.
+                    }
+                    specialize (H5 k1 H2).
+                    KeyFacts.order.
+              -- pose proof (Znth_In (c') (map Some ((k0, e) :: t)) ltac:(rewrite Zlength_map; omega)).
+                 rewrite Heqn in H2.
+                 clear - H2.
+                 exfalso.
+                 simpl in H2.
+                 inv H2; [congruence | ].
+                 induction t.
+                 ++ inv H.
+                 ++ apply IHt.
+                    inv H; congruence.
+      Qed.
+
+      Lemma get_in_weak: forall k v c t,
+          abs_rel c t ->
+          get c t = Some (k, v) ->
+          In (k, v) t.
+      Proof.
+        intros.
+        inv H.
+        unfold get in H0.
+        assert (c <> Zlength t). {
+          intro.
+          subst.
+          rewrite Znth_overflow in H0 by (rewrite Zlength_map; omega).
+          inv H0.
+        }
+        pose proof (Znth_In c (map Some t) ltac:(change (cursor elt) with Z in *; rewrite Zlength_map; omega)).
+        rewrite H0 in H3.
+        clear -H3.
+        induction t as [ | [] ?].
+        - inv H3.
+        - inv H3.
+          + inv H.
+            left.
+            auto.
+          + right.
+            auto.
+      Qed.
+
+      Theorem get_in: forall k v c t,
+        abs_rel c t ->
+        key_rel k c t ->
+        In (k, v) t <->
+        get c t = Some (k, v).
+      Proof.
+        intros k v c t.
+        generalize dependent k.
+        generalize dependent v.
+        generalize dependent c.
+        induction t as [ | [] ?]; intros; split; intros.
+        - inv H1.
+        - unfold get in H1.
+          simpl in H1.
+          rewrite Znth_nil in H1.
+          inv H1.
+        - destruct (KeyType.eq_dec k k0) as [Heq | Heq]; change (KeyType.eq k k0) with (k = k0) in Heq.
+          + subst.
+            destruct (eq_dec c 0).
+            * subst. unfold get.
+              simpl.
+              rewrite Znth_0_cons.
+              f_equal.
+              inv H.
+              apply table_correct_strong in H2.
+              inv H2.
+              inv H1.
+              -- assumption.
+              -- rewrite Forall_forall in H6.
+                 apply in_map with (f := fst) in H.
+                 apply H6 in H.
+                 simpl in H.
+                 KeyFacts.order.
+            * unfold key_rel in H0.
+              specialize (H0 0) as [? _].
+              inv H.
+              specialize (H0 ltac:(change (cursor elt) with Z in *; omega)) as [k' []].
+              unfold get_key, get in H.
+              simpl in H.
+              inv H.
+              KeyFacts.order.
+          + destruct (eq_dec c 0).
+            * subst.
+              exfalso.
+              unfold key_rel in H0.
+              inv H.
+              (* [k < k0], [in_nth] *)
+              apply table_correct_strong in H2.
+              inv H2.
+              assert (KeyType.lt k k0). {
+                rewrite Forall_forall in H6.
+                apply in_map with (f := fst) in H1.
+                simpl in H1.
+                inv H1; [congruence | ].
+                apply H6 in H.
+                assumption.
+              }
+              specialize (H0 0) as [_ ?].
+              specialize (H0 ltac:(list_solve)) as [k' []].
+              unfold get_key, get in H0.
+              simpl in H0.
+              inv H0.
+              KeyFacts.order.
+            * unfold get.
+              simpl.
+              inv H.
+              rewrite Znth_pos_cons by (change (cursor elt) with Z in *; omega).
+              apply IHt.
+              -- apply table_correct_strong in H2.
+                 inv H2.
+                 apply table_correct_strong in H5.
+                 split; [ assumption | ].
+                 change (cursor elt) with Z in *.
+                 rewrite Zlength_cons in H3.
+                 list_solve.
+              -- unfold key_rel in *.
+                 intros; split; intros.
+                 ++ specialize (H0 (c' + 1)) as [? _].
+                    change (cursor elt) with Z in *.
+                    specialize (H0 ltac:(omega)) as [k' []].
+                    exists k'.
+                    unfold get_key, get in H0.
+                    simpl in H0.
+                    rewrite Znth_pos_cons in H0 by omega.
+                    replace (c' + 1 - 1) with c' in H0 by omega.
+                    auto.
+                 ++ specialize (H0 (c' + 1)) as [_ ?].
+                    change (cursor elt) with Z in *.
+                    rewrite Zlength_cons in *.
+                    specialize (H0 ltac:(omega)) as [k' []].
+                    exists k'.
+                    unfold get_key, get in H0.
+                    simpl in H0.
+                    rewrite Znth_pos_cons in H0 by omega.
+                    replace (c' + 1 - 1) with c' in H0 by omega.
+                    auto.
+              -- inv H1; congruence.
+        - unfold get in H1.
+          inv H.
+          assert (c <> Zlength ((k, e) :: t)). {
+            intro.
+            rewrite Znth_overflow in H1 by
+                (rewrite Zlength_map; change (cursor elt) with Z in *; omega).
+            inv H1.
+          }
+          pose proof (Znth_In c (map Some ((k, e) :: t))
+                              ltac:(rewrite Zlength_map; change (cursor elt) with Z in *; omega)).
+          rewrite H1 in H4.
+          clear -H4.
+          inv H4.
+          + inv H.
+            left.
+            auto.
+          + right.
+            induction t.
+            * inv H.
+            * inv H.
+              -- left.
+                 congruence.
+              -- right.
+                 auto.
+      Qed.
+
+      (* permute of get and insert operations *)
+      (* Assume [key_rel] does entail [abs_rel] *)
+      Theorem get_put_same: forall t c1 c2 k e a,
+          abs_rel c1 (fst (snd (put k e c2 (t, a)))) ->
+          abs_rel c2 t ->
+          key_rel k c1 (fst (snd (put k e c2 (t, a)))) ->
+          get c1 (fst (snd (put k e c2 (t, a)))) = Some (k, e).
+      Proof.
+        intros t c1 c2 k e a.
+        generalize dependent c1.
+        generalize dependent c2.
+        generalize dependent k.
+        generalize dependent e.
+        generalize dependent a.
+        induction t as [ | [] ?]; intros.
+        - simpl.
+          simpl in H.
+          inv H.
+          rewrite Zlength_cons in H3.
+          simpl in H3.
+          simpl in H1.
+          assert (c1 = 0 \/ c1 = 1) by (change (cursor elt) with Z in *; omega).
+          destruct H; subst.
+          + reflexivity.
+          + unfold key_rel in H1.
+            specialize (H1 0) as [? _].
+            specialize (H ltac:(omega)) as [? []].
+            unfold get_key, get in H.
+            simpl in H.
+            inv H.
+            KeyFacts.order.
+        - simpl.
+          simpl put in *.
+          repeat if_tac.
+          + destruct (eq_dec c1 0).
+            * subst.
+              unfold get.
+              reflexivity.
+            * unfold key_rel in H1.
+              specialize (H1 0) as [? _].
+              inv H.
+              specialize (H1 ltac:(change (cursor elt) with Z in *; omega)) as [? []].
+              simpl in H.
+              unfold get_key, get in H.
+              simpl in H.
+              inv H.
+              KeyFacts.order.
+          + subst.
+            destruct (eq_dec c1 0).
+            * subst.
+              reflexivity.
+            * unfold key_rel in H1.
+              specialize (H1 0) as [? _].
+              inv H.
+              specialize (H1 ltac:(change (cursor elt) with Z in *; omega)) as [? []].
+              inv H.
+              KeyFacts.order.
+          + unfold put in IHt.
+            specialize (IHt a e0 k0 0 (c1 - 1)).
+            destruct (eq_dec c1 0).
+            * subst.
+              unfold key_rel in H1.
+              specialize (H1 0) as [_ ?].
+              simpl in H1.
+              rewrite Zlength_cons in H1.
+              specialize (H1 ltac:(change (cursor elt) with Z in *; list_solve)) as [? []].
+              unfold get_key, get in H1.
+              simpl in H1.
+              inv H1.
+              KeyFacts.order.
+            * unfold get.
+              simpl.
+              inv H.
+              rewrite Znth_pos_cons by (change (cursor elt) with Z in *; omega).
+              unfold get in IHt.
+              simpl in IHt.
+              apply IHt.
+              -- split.
+                 ++ simpl in H4.
+                    apply table_correct_strong in H4.
+                    inv H4.
+                    apply table_correct_strong in H7.
+                    assumption.
+                 ++ simpl in H5.
+                    rewrite Zlength_cons in H5.
+                    change (cursor elt) with Z in *.
+                    omega.
+              -- split.
+                 ++ inv H0.
+                    apply table_correct_strong in H.
+                    inv H.
+                    apply table_correct_strong in H8.
+                    assumption.
+                 ++ list_solve.
+              -- split; intros.
+                 ++ unfold key_rel in H1.
+                    specialize (H1 (c' + 1)) as [? _].
+                    specialize (H1 ltac:(omega)) as [k' []].
+                    exists k'.
+                    unfold get_key, get in *.
+                    simpl in *.
+                    rewrite Znth_pos_cons in H1 by omega.
+                    replace (c' + 1 - 1) with c' in H1 by omega.
+                    auto.
+                 ++ unfold key_rel in H1.
+                    specialize (H1 (c' + 1)) as [_ ?].
+                    simpl in *.
+                    rewrite Zlength_cons in H1.
+                    specialize (H1 ltac:(omega)) as [k' []].
+                    exists k'.
+                    unfold get_key, get in *.
+                    simpl in *.
+                    rewrite Znth_pos_cons in H1 by (change (cursor elt) with Z in *; omega).
+                    replace (c' + 1 - 1) with c' in H1 by omega.
+                    auto.
+      Qed.
+
+      Lemma key_rel_0': forall k1 k2 e t,
+          ~ KeyType.lt k1 k2 ->
+          table_correct ((k1, e) :: t) ->
+          key_rel k2 0 ((k1, e) :: t).
+      Proof.
+        intros.
+        split; intros.
+        - omega.
+        - assert (exists kv, get c' ((k1, e) :: t) = Some kv). {
+            apply get_inrange.
+            - split; [ auto | omega ].
+            - unfold eq_cursor, last_cursor.
+              change (cursor elt) with Z in *.
+              omega.
+          }
+          destruct H2 as [[k' v'] ?].
+          apply table_correct_strong in H0.
+          inv H0.
+          eexists.
+          split.
+          + unfold get_key.
+            rewrite H2.
+            reflexivity.
+          + destruct (KeyType.eq_dec k1 k'); change (KeyType.eq k1 k') with (k1 = k') in *.
+            * subst.
+              KeyFacts.order.
+            * destruct (eq_dec c' 0).
+              -- subst.
+                 inv H2.
+                 congruence.
+              -- unfold get in H2.
+                 simpl in H2.
+                 rewrite Znth_pos_cons in H2 by omega.
+                 assert (abs_rel (c' - 1) t). {
+                   split.
+                   - apply table_correct_strong.
+                     assumption.
+                   - rewrite Zlength_cons in H1.
+                     list_solve.
+                 }
+                 assert (In (k', v') t). {
+                   apply get_in_weak with (c := c' - 1).
+                   - assumption.
+                   - unfold get.
+                     assumption.
+                 }
+                 rewrite Forall_forall in H6.
+                 apply in_map with (f := fst) in H3.
+                 simpl in H3.
+                 apply H6 in H3.
+                 KeyFacts.order.
+      Qed.
+
+      Lemma key_rel_0: forall k e t,
+          table_correct ((k, e) :: t) ->
+          key_rel k 0 ((k, e) :: t).
+      Proof.
+        intros.
+        split; intros.
+        - omega.
+        - assert (exists kv, get c' ((k, e) :: t) = Some kv). {
+            apply get_inrange.
+            - split; [ auto | omega ].
+            - unfold eq_cursor, last_cursor.
+              change (cursor elt) with Z in *.
+              omega.
+          }
+          destruct H1 as [[k' v'] ?].
+          apply table_correct_strong in H.
+          inv H.
+          eexists.
+          split.
+          + unfold get_key.
+            rewrite H1.
+            reflexivity.
+          + destruct (KeyType.eq_dec k k'); change (KeyType.eq k k') with (k = k') in *.
+            * subst.
+              KeyFacts.order.
+            * destruct (eq_dec c' 0).
+              -- subst.
+                 inv H1.
+                 congruence.
+              -- unfold get in H1.
+                 simpl in H1.
+                 rewrite Znth_pos_cons in H1 by omega.
+                 assert (abs_rel (c' - 1) t). {
+                   split.
+                   - apply table_correct_strong.
+                     assumption.
+                   - rewrite Zlength_cons in H0.
+                     omega.
+                 }
+                 assert (In (k', v') t). {
+                   apply get_in_weak with (c := c' - 1).
+                   - assumption.
+                   - unfold get.
+                     assumption.
+                 }
+                 rewrite Forall_forall in H5.
+                 apply in_map with (f := fst) in H2.
+                 simpl in H2.
+                 apply H5 in H2.
+                 KeyFacts.order.
+      Qed.
+
+      Theorem get_key_rel: forall k c t,
+          abs_rel c t ->
+          get_key c t = Some k ->
+          key_rel k c t.
+      Proof.
+        (* intros k c t. *)
+        (* generalize dependent c. *)
+        (* induction t as [ | [] ? ]; intros. *)
+        (* - unfold get_key, get in H0. *)
+        (*   simpl in H0. *)
+        (*   rewrite Znth_nil in H0. *)
+        (*   inv H0. *)
+        (* - destruct (eq_dec c 0). *)
+        (*   + subst. *)
+        (*     unfold get_key, get in H0. *)
+        (*     inv H0. *)
+        (*     split; intros. *)
+        (*     * omega. *)
+        (*     * assert (exists kv, get c' ((k, e) :: t) = Some kv). { *)
+        (*         apply get_inrange. *)
+        (*         - inv H. *)
+        (*           split; [auto | omega]. *)
+        (*         - unfold eq_cursor, last_cursor. *)
+        (*           change (cursor elt) with Z in *. *)
+        (*           omega. *)
+        (*       } *)
+        (*       destruct H1 as [[] ]. *)
+        (*       exists k0. *)
+        (*       unfold get_key. *)
+        (*       rewrite H1. *)
+        (*       inv H. *)
+        (*       apply get_in_weak in H1; [ | split; [ auto | omega ]]. *)
+        (*       apply table_correct_strong in H2. *)
+        (*       inv H2. *)
+        (*       rewrite Forall_forall in H6. *)
+        (*       inv H1. *)
+        (*       -- inv H. *)
+        (*          auto. *)
+        (*       -- apply in_map with (f := fst) in H. *)
+        (*          apply H6 in H. *)
+        (*          simpl in H. *)
+        (*          split; [ auto | KeyFacts.order ]. *)
+        (*   + specialize (IHt (c - 1)). *)
+        (*     assert (abs_rel (c - 1) t). { *)
+        (*       split. *)
+        (*       - inv H. *)
+        (*         apply table_correct_strong in H1. *)
+        (*         inv H1. *)
+        (*         apply table_correct_strong in H4. *)
+        (*         assumption. *)
+        (*       - inv H. *)
+        (*         rewrite Zlength_cons in H2. *)
+        (*         change (cursor elt) with Z in *. *)
+        (*         omega. *)
+        (*     } *)
+        (*     unfold get_key, get in *. *)
+        (*     simpl in H0. *)
+        (*     inv H. *)
+        (*     rewrite Znth_pos_cons in H0 by (change (cursor elt) with Z in *; omega). *)
+        (*     specialize (IHt H1 H0). *)
+        (*     split; intros. *)
+        (*     * destruct (eq_dec c' 0). *)
+        (*       -- subst. *)
+        (*          exists k0. *)
+        (*          split; [auto | ]. *)
+      Admitted.
+
+      Theorem get_eq (t1 t2: table elt):
+        table_correct t1 ->
+        table_correct t2 ->
+        (forall k c1 c2,
+            key_rel k c1 t1 ->
+            abs_rel c1 t1 ->
+            key_rel k c2 t2 ->
+            abs_rel c2 t2 ->
+            get c1 t1 = get c2 t2)
+        -> t1 = t2.
+      Proof.
+        generalize dependent t2.
+        induction t1 as [ | [] ?]; intros.
+        - destruct t2 as [ | [] ?].
+          + reflexivity.
+          + specialize (H1 k 0 0).
+            assert (key_rel k 0 []). {
+              split; intros.
+              - omega.
+              - rewrite Zlength_nil in H2.
+                omega.
+            }
+            assert (abs_rel 0 []). {
+              split; intros.
+              - assumption.
+              - rewrite Zlength_nil.
+                omega.
+            }
+            assert (key_rel k 0 ((k, e) :: t2)). {
+              apply key_rel_0.
+              assumption.
+            }
+            assert (abs_rel 0 ((k, e) :: t2)). {
+              split; intros.
+              - assumption.
+              - list_solve.
+            }
+            specialize (H1 H2 H3 H4 H5).
+            inv H1.
+        - destruct t2 as [ | [] ?].
+          + specialize (H1 k 0 0).
+            assert (key_rel k 0 ((k, e) :: t1)). {
+              apply key_rel_0.
+              assumption.
+            }
+            assert (abs_rel 0 ((k, e) :: t1)). {
+              split; intros.
+              - assumption.
+              - list_solve.
+            }
+            assert (key_rel k 0 []). {
+              split; intros.
+              - omega.
+              - rewrite Zlength_nil in H4.
+                omega.
+            }
+            assert (abs_rel 0 []). {
+              split; intros.
+              - assumption.
+              - rewrite Zlength_nil.
+                omega.
+            }
+            specialize (H1 H2 H3 H4 H5).
+            inv H1.
+          + remember (if KeyFacts.lt_dec k k0 then k else k0) as k'.
+            assert (key_rel k' 0 ((k, e) :: t1)). {
+              apply key_rel_0'.
+              - if_tac in Heqk'; subst; KeyFacts.order.
+              - assumption.
+            }
+            assert (abs_rel 0 ((k, e) :: t1)). {
+              split; intros.
+              - assumption.
+              - list_solve.
+            }
+            assert (key_rel k' 0 ((k0, e0) :: t2)). {
+              apply key_rel_0'.
+              - if_tac in Heqk'; subst; KeyFacts.order.
+              - assumption.
+            }
+            assert (abs_rel 0 ((k0, e0) :: t2)). {
+              split; intros.
+              - assumption.
+              - list_solve.
+            }
+            pose proof (H1 _ _ _ H2 H3 H4 H5).
+            inv H6.
+            f_equal.
+            destruct (nil_or_non_nil t1); destruct (nil_or_non_nil t2); subst.
+            * unfold get.
+              simpl.
+              rewrite ?Znth_nil.
+              reflexivity.
+            * destruct t2 as [ | [] ?]; [ congruence | ].
+              clear n.
+              specialize (H1 k 1 1).
+              assert (KeyFacts.TO.lt k0 k). {
+                inv H5.
+                apply table_correct_strong in H6.
+                inv H6.
+                inv H10.
+                assumption.
+              }
+              assert (key_rel k 1 [(k0, e0)]). {
+                split; intros.
+                + assert (c' = 0) by omega.
+                  subst.
+                  exists k0.
+                  split; auto.
+                + change (Zlength _) with 1 in H7.
+                  omega.
+              }
+              assert (abs_rel 1 [(k0, e0)]). {
+                split; [auto | change (Zlength _) with 1; omega].
+              }
+              assert (key_rel k 1 ((k0, e0) :: (k, e) :: t2)). {
+                split; intros.
+                + assert (c' = 0) by omega.
+                  subst.
+                  exists k0.
+                  split; auto.
+                + pose proof (get_inrange
+                                c'
+                                ((k0, e0) :: (k, e) :: t2)
+                                ltac:(split; [ auto | omega])
+                                ltac:(unfold eq_cursor, last_cursor; change (cursor elt) with Z in *; omega)).
+                  destruct H10 as [[] ?].
+                  exists k1.
+                  unfold get_key.
+                  rewrite H10.
+                  unfold get in H10.
+                  simpl in H10.
+                  rewrite Znth_pos_cons in H10 by omega.
+                  assert (abs_rel (c' - 1) ((k, e) :: t2)). {
+                    split.
+                    - inv H5.
+                      apply table_correct_strong in H11.
+                      inv H11.
+                      apply table_correct_strong.
+                      assumption.
+                    - rewrite ?Zlength_cons in *.
+                      list_solve.
+                  }
+                  pose proof (get_in_weak k1 e1 (c' -1) ((k, e) :: t2) H11 H10).
+                  inv H5.
+                  apply table_correct_strong in H13.
+                  inv H13.
+                  inv H16.
+                  rewrite Forall_forall in H18.
+                  apply in_map with (f := fst) in H12.
+                  simpl in H12.
+                  destruct H12; auto.
+              }
+              assert (abs_rel 1 ((k0, e0) :: (k, e) :: t2)). {
+                split; [auto | list_solve].
+              }
+              specialize (H1 H7 H8 H9 H10).
+              inv H1.
+            * destruct t1 as [ | [] ?]; [ congruence | ].
+              clear n.
+              specialize (H1 k 1 1).
+              assert (KeyFacts.TO.lt k0 k). {
+                inv H3.
+                apply table_correct_strong in H6.
+                inv H6.
+                inv H10.
+                assumption.
+              }
+              assert (key_rel k 1 [(k0, e0)]). {
+                split; intros.
+                + assert (c' = 0) by omega.
+                  subst.
+                  exists k0.
+                  split; auto.
+                + change (Zlength _) with 1 in H7.
+                  omega.
+              }
+              assert (abs_rel 1 [(k0, e0)]). {
+                split; [auto | change (Zlength _) with 1; omega].
+              }
+              assert (key_rel k 1 ((k0, e0) :: (k, e) :: t1)). {
+                split; intros.
+                + assert (c' = 0) by omega.
+                  subst.
+                  exists k0.
+                  split; auto.
+                + pose proof (get_inrange
+                                c'
+                                ((k0, e0) :: (k, e) :: t1)
+                                ltac:(split; [ auto | omega])
+                                ltac:(unfold eq_cursor, last_cursor; change (cursor elt) with Z in *; omega)).
+                  destruct H10 as [[] ?].
+                  exists k1.
+                  unfold get_key.
+                  rewrite H10.
+                  unfold get in H10.
+                  simpl in H10.
+                  rewrite Znth_pos_cons in H10 by omega.
+                  assert (abs_rel (c' - 1) ((k, e) :: t1)). {
+                    split.
+                    - inv H3.
+                      apply table_correct_strong in H11.
+                      inv H11.
+                      apply table_correct_strong.
+                      assumption.
+                    - rewrite ?Zlength_cons in *.
+                      list_solve.
+                  }
+                  pose proof (get_in_weak k1 e1 (c' -1) ((k, e) :: t1) H11 H10).
+                  inv H3.
+                  apply table_correct_strong in H13.
+                  inv H13.
+                  inv H16.
+                  rewrite Forall_forall in H18.
+                  apply in_map with (f := fst) in H12.
+                  simpl in H12.
+                  destruct H12; auto.
+              }
+              assert (abs_rel 1 ((k0, e0) :: (k, e) :: t1)). {
+                split; [auto | list_solve].
+              }
+              specialize (H1 H9 H10 H7 H8).
+              inv H1.
+            * apply IHt1.
+              -- apply table_correct_strong in H.
+                 inv H.
+                 apply table_correct_strong.
+                 assumption.
+              -- apply table_correct_strong in H0.
+                 inv H0.
+                 apply table_correct_strong.
+                 assumption.
+              -- intros.
+                 destruct t1 as [ | [] ? ]; destruct t2 as [ | [] ? ]; try congruence.
+                 clear H4 H2 H3 H5 n n0.
+                 destruct (KeyFacts.lt_dec k k0).
+                 ++ remember (if KeyFacts.lt_dec k1 k2 then k1 else k2) as k'.
+                    specialize (H1 k' 1 1).
+                    admit.
+                 ++ admit.
+      Admitted.
+      
+      Theorem get_put_diff:
+        k1 <> k2 ->
+        table_correct t ->
+        cursor_correct c2 ->
+        key_rel k1 c1 (fst (snd (put k2 e c2 (t, a)))) ->
+        key_rel k1 c3 t ->
+        get c1 (fst (snd (put k2 e c2 (t, a)))) = get c3 t.
+      Proof.
+      Admitted.
+
+      (* get in specific conditions *)
+      Axiom get_last:
+        get (last_cursor t) t = None.
+      Axiom get_empty: 
+        abs_rel c (fst (empty a)) -> get c (fst (empty a)) = None.
+
+      (* Cursor creation and keys *)
+ 
+      Axiom make_cursor_key:
+        key_rel k (make_cursor k t) t.
+      (* Axiom move_cursor_key: *)
+      (*   key_rel k (move_cursor k c t) t. *)
+
+      (* cursor movement with respect to the order of key *)
+      Axiom next_prev:
+        abs_rel c t -> ~ eq_cursor c (last_cursor t) t -> eq_cursor c (prev_cursor (next_cursor c t) t) t.
+      Axiom prev_next:
+        abs_rel c t -> ~ eq_cursor c (first_cursor t) t -> eq_cursor c (next_cursor (prev_cursor c t) t) t.
+      Axiom next_order:
+        ~ eq_cursor c (last_cursor t) t -> key_rel k1 c t -> key_rel k2 (next_cursor c t) t -> KeyType.lt k1 k2.
+      Axiom prev_order:
+        ~ eq_cursor c (first_cursor t) t -> key_rel k1 c t -> key_rel k2 (prev_cursor c t) t -> KeyType.lt k2 k1.
+      (* TODO: does this definition work? *)
+      Axiom next_compact:
+        ~ eq_cursor c (last_cursor t) t ->
+        key_rel k1 c t -> key_rel k2 (next_cursor c t) t ->
+        ~ key_rel k3 c t -> KeyType.lt k1 k3 /\ KeyType.lt k3 k2.
+      Axiom prev_compact:
+        ~ eq_cursor c (first_cursor t) t ->
+        key_rel k1 c t -> key_rel k2 (prev_cursor c t) t ->
+        ~ key_rel k3 c t -> KeyType.lt k2 k3 /\ KeyType.lt k3 k1.
+    End Specs.
+  End Types.
+
 Module Type CONCRETE_TABLE (KeyType: UsualOrderedType) <: ABSTRACT_TABLE KeyType.
   (* A concrete table requires all the features of an abstract table
    * (actually not, it does not require parametrized value), and additionally, it requires some rep predicates *)
@@ -127,44 +1210,12 @@ Module Type CONCRETE_TABLE (KeyType: UsualOrderedType) <: ABSTRACT_TABLE KeyType
   Definition elt: Type := val.
 
   Parameter table_rep: table elt -> val -> mpred.
+  (* should [cursor_rep] be some form of magic wand exposed to client, or just leave it there? *)
   Parameter cursor_rep: cursor elt -> table elt -> val -> mpred.
-  Section Specs.
-    Variable ttable tcursor: type.
-    Definition new_cursor: funspec :=
-      WITH t: table elt, pt: val
-      PRE [ 1%positive OF tptr ttable ]
-      PROP (table_correct t)
-      LOCAL (temp 1%positive pt)
-      SEP (table_rep t pt)
-      POST [ tptr tcursor ]
-      EX p': val, EX c: cursor elt,
-      PROP (eq_cursor (first_cursor t) c t)
-      LOCAL (temp ret_temp p')
-      SEP (table_rep t pt; cursor_rep c t p').
-
-    (* TODO: should I define what property is expected here? *)
-    (* thing like:
-     * [
-          WITH t: table elt, c: cursor elt, v: elt,
-               pt: val, pc: val
-          PRE [_table OF tptr ttable, _cursor OF tptr tcursor]
-          PROP (get c t = Some v)
-          LOCAL (local _table pt; local _cursor pc)
-          SEP (table_rep t pt; cursor_rep t pc)
-          POST [ telt ]
-          PROP ()
-          LOCAL (local ret_temp v)
-          SEP (table_rep t pt; cursor_rep t pc)
-          ]
-     *)
-    (* problems: the return type telt cannot be determined well *)
-
-    (* TODO: do we always need two instance of such module? One for the abstract model one for the rep relation? *)
-  End Specs.
 End CONCRETE_TABLE.
 
 (* For now, only usual ordered types are proved to be flattenable *)
-Module Type FLATTENABLE_CONCRETE_TABLE (KeyType: UsualOrderedType) <: ABSTRACT_TABLE KeyType.
+Module Type FLATTENABLE_TABLE (KeyType: UsualOrderedType) <: ABSTRACT_TABLE KeyType.
   Include ABSTRACT_TABLE KeyType.
   Module Flattened := SortedListTable KeyType.
   Section Spec.
@@ -173,21 +1224,29 @@ Module Type FLATTENABLE_CONCRETE_TABLE (KeyType: UsualOrderedType) <: ABSTRACT_T
     Axiom flatten_invariant: forall t,
         Flattened.sorted (flatten t) /\
         forall (k: key) (c: cursor elt), key_rel k c t -> get c t = Flattened.get k (flatten t).
+  End Spec.
+End FLATTENABLE_TABLE.
 
-    Theorem put_permute (k: key) (v: elt) (c: cursor elt) (t: table elt):
-      key_rel k c t ->
-      flatten (snd (put c v t)) = Flattened.put k v (flatten t).
+
+
+Module FlattenableTableFacts (KeyType: UsualOrderedType) (FlattenableTable: FLATTENABLE_TABLE KeyType).
+  Include FlattenableTable.
+  Section Implication.
+    Context {elt: Type}.
+    Theorem put_permute (k: key) (v: elt) (c: cursor elt) (t: table elt) (l: list val):
+      cursor_correct c ->
+      flatten (snd (put k v l c t)) = Flattened.put k v (flatten t).
     Proof.
-      pose proof flatten_invariant.
+      pose proof (@flatten_invariant elt).
       intros.
       apply Flattened.get_eq.
       - intros.
         pose proof H.
-        specialize (H (snd (put c v t))).
+        specialize (H (snd (put k v l c t))).
         inv H.
-        pose (c' := make_cursor k (snd (put c v t))).
-        pose proof (make_cursor_key (snd (put c v t)) k).
-        pose (c'' := make_cursor k0 (snd (put c v t))).
+        pose (c' := make_cursor k (snd (put k v l c t))).
+        pose proof (make_cursor_key (snd (put k v l c t)) k).
+        pose (c'' := make_cursor k0 (snd (put k v l c t))).
         specialize (H3 k0 c'' ltac:(apply make_cursor_key; auto)).
         rewrite <- H3.
         destruct (KeyType.eq_dec k k0); change (KeyType.eq k k0) with (k = k0) in *.
@@ -203,7 +1262,7 @@ Module Type FLATTENABLE_CONCRETE_TABLE (KeyType: UsualOrderedType) <: ABSTRACT_T
             apply make_cursor_key.
           * apply make_cursor_key.
           * apply make_cursor_key.
-      - specialize (H (snd (put c v t))).
+      - specialize (H (snd (put k v l c t))).
         inv H.
         assumption.
       - apply Flattened.put_sorted.
@@ -211,5 +1270,5 @@ Module Type FLATTENABLE_CONCRETE_TABLE (KeyType: UsualOrderedType) <: ABSTRACT_T
         inv H.
         assumption.
     Qed.
-  End Spec.
-End FLATTENABLE_CONCRETE_TABLE.
+  End Implication.
+End FlattenableTableFacts.
